\documentclass[12pt,a4paper]{article}
\usepackage{geometry}
\geometry{left=2.5cm,right=2.5cm,top=2.0cm,bottom=2.5cm}
\usepackage[english]{babel}
\usepackage{amsmath,amsthm}
\usepackage{amsfonts}
\usepackage[longend,ruled,linesnumbered]{algorithm2e}
\usepackage{fancyhdr}
\usepackage{ctex}
\usepackage{array}
\usepackage{listings}
\usepackage{color}
\usepackage{graphicx}
\newtheorem{theorem}{定理}
\newtheorem{lemma}[theorem]{引理}
\newtheorem{corollary}[theorem]{推论}


\begin{document}
	
	\noindent
	
\section{时域卷积定理}	

	\begin{theorem}[时域卷积定理]
		
			若$F_1(j w) = F[f_1(t)], F_2(j w) = F[f_2(t)]$, 则$$F\left[f_1(t) \star f_2(t)\right]=F_1(j w) F_2(j w)$$
	\end{theorem}
	
	\begin{proof}[证明]
		\begin{equation*}
			\begin{aligned}
				F\left[f_1(t) \star f_2(t)\right] & =\int_{-\infty}^{+\infty} \int_{-\infty}^{+\infty}\left[f_1(t) \star f_2(t)\right] e^{-j w t} d t d \tau \\
				& =\int_{-\infty}^{+\infty} \int_{-\infty}^{+\infty} f_1(\tau) f_2(t-\tau) e^{-j w t} d t d \tau \\
				& =\int_{-\infty}^{+\infty} f_1(\tau) d \tau\left[\int_{-\infty}^{+\infty} f_2(t-\tau) e^{-j w t} d t\right] \\
				& =F_2(j w)\left[\int_{-\infty}^{+\infty} f_1(\tau) e^{-j w \tau} d \tau\right] \\
				& =F_1(j w) F_2(j w)
			\end{aligned}
		\end{equation*}
	\end{proof}
	
\section{频域卷积定理}
	\begin{theorem}[频域卷积定理]
		$$
		F[f_1(t)f_2(t)] = \frac{1}{2\pi} F_1(j w) \star F_2(j w)
		$$
	\end{theorem}
	
	\begin{proof}[证明]
		\begin{equation*}
			\begin{aligned}
				F^{-1}\left[F_1(j w) \star F_2(j w)\right] & =\frac{1}{2 \pi} \int_{-\infty}^{+\infty}\left[F_1(j w) \star F_2(j w)\right] e^{j w t} d w \\
				& =\frac{1}{2 \pi} \int_{-\infty}^{+\infty} \int_{-\infty}^{+\infty}\left[F_1(j u) F_2(j(w-u))\right] e^{j w t} d w d u \\
				& =\int_{-\infty}^{+\infty} F_1(j u) d u\left[\frac{1}{2 \pi} \int_{-\infty}^{+\infty} F_2(j(w-u)) e^{j w t} d w\right] \\
				& =\int_{-\infty}^{+\infty} F_1(j u) e^{j u t} d u\left[\frac{1}{2 \pi} \int_{-\infty}^{+\infty} F_2(j(w-u)) e^{j w t} d w\right] \\
				& =2 \pi f_2(t)\left[\frac{1}{2 \pi} \int_{-\infty}^{+\infty} F_1(j u) e^{j u t} d u\right] \\
				& =2 \pi f_1(t) f_2(t)
			\end{aligned}
		\end{equation*}
	\end{proof}
\end{document}
